@prefix dct: <http://purl.org/dc/terms/> .
@prefix ex: <http://example.org/persian-architecture/> .
@prefix iiif: <http://iiif.io/api/presentation/2#> .
@prefix owl: <http://www.w3.org/2002/07/owl#> .
@prefix rdf: <http://www.w3.org/1999/02/22-rdf-syntax-ns#> .
@prefix rdfs: <http://www.w3.org/2000/01/rdf-schema#> .
@prefix sc: <http://purl.org/science/owl/sciencecommons/> .
@prefix schema: <http://schema.org/> .
@prefix skos: <http://www.w3.org/2004/02/skos/core#> .
@prefix tgn: <http://vocab.getty.edu/tgn/> .
@prefix prefix: <http://qudt.org/vocab/prefix/> . # QUDT Prefixes Version 2.1 Vocabulary
@prefix xsd: <http://www.w3.org/2001/XMLSchema#> .
@prefix mdhn: <http://example.com/mdhn/> .

# Ontology Definition
mdhn:PersianArchitectureOntology a owl:Ontology ;
    dct:title "Persian Architecture Ontology"@en ;
    dct:description "An ontology for Persian architectural landmarks and associated high-level IIIF images and slides, integrated with Schema.org."@en .

# Classes
mdhn:CHABuilding a owl:Class ;
    rdfs:subClassOf schema:LandmarkOrHistoricalBuilding ;
    rdfs:label "Cultural Heritage Architectural Building"@en ;
    rdfs:comment "A significant architectural site or historical building in Persian architecture."@en .

mdhn:VisualArtwork a owl:Class ;
    rdfs:subClassOf schema:VisualArtwork ;
    rdfs:label "Visual Artwork"@en ;
    rdfs:comment "Digital resources such as IIIF images or slides representing Persian architectural landmarks."@en .

mdhn:DCHTypeTaxon a owl:Class ;
    rdfs:subClassOf skos:Concept ;
    rdfs:label "Digital cultural heritage object type Taxon"@en ;
    rdfs:comment "Indicating type of digital cultural heritage objects"@en .
mdhn:SubjectTerm a owl:Class ;
    rdfs:subClassOf sc:DefinedTerm ;
    rdfs:label "Subject Defined Term"@en ;
    rdfs:comment "A thesaurus subject representing subjects or themes related to Persian architecture (e.g., domes, arches, tilework)."@en .

mdhn:SpatialTGNTerm a owl:Class ;
    rdfs:subClassOf sc:DefinedTerm ;
    rdfs:label "Spatial TGN Term"@en ;
    rdfs:comment "A thesaurus term based on TGN representing spatial info  related to architectural site"@en .    


# Properties

mdhn:containsCHABuilding a owl:ObjectProperty ;
    rdfs:domain mdhn:SpatialTGNTerm ;
    rdfs:range mdhn:CHABuilding ;
    owl:inverseOf mdhn:hasTGNSpatial ;
    rdfs:label "contains cultural heritage architectural building"@en ;
    rdfs:comment "Links a vuilding to"@en .

mdhn:hasTGNSpatial a owl:ObjectProperty ;
    rdfs:domain mdhn:CHABuilding ;
    rdfs:range mdhn:SpatialTGNTerm ;
    rdfs:label "has TGN spatial"@en ;
    rdfs:comment "Links a CHA building to a TGN concept"@en .  

mdhn:hasDCHType a owl:ObjectProperty ;
    rdfs:domain mdhn:VisualArtwork ;
    rdfs:range mdhn:DCHTypeTaxon;
    rdfs:label "has DCH type"@en ;
    rdfs:comment "Links a DCH object to type"@en .
mdhn:hasInstances a owl:ObjectProperty ;
    rdfs:domain mdhn:DCHTypeTaxon ;
    rdfs:range mdhn:VisualArtwork;
    owl:inverseOf mdhn:hasDCHType ;
    rdfs:label "has Instances"@en ;
    rdfs:comment "Links a DCH object type to assoxiated instanxes"@en .              

mdhn:hasDigitalObject a owl:ObjectProperty ;
    rdfs:domain mdhn:CHABuilding ;
    rdfs:range mdhn:VisualArtwork ;
    rdfs:label "has related Digital object"@en ;
    rdfs:comment "Links a landmark or historical building to its digital visual/linguistic representations (e.g., IIIF images or slides)."@en .


mdhn:hasDepicts a owl:ObjectProperty ;
    owl:inverseOf mdhn:hasDigitalObject ;
    rdfs:domain mdhn:VisualArtwork;
    rdfs:range mdhn:CHABuilding  ;
    rdfs:label "has depicts a concept"@en ;
    rdfs:comment "Associates a digital object to a CHA building."@en .
    
mdhn:hasSubject a owl:ObjectProperty ;
    rdfs:domain mdhn:VisualArtwork ;
    rdfs:range mdhn:SubjectTerm ;
    rdfs:label "has subject"@en ;
    rdfs:comment "Associates a visual artwork with a subject taxon (e.g., architectural feature like iwan or minaret)."@en .

mdhn:subjectRelatesTo a owl:ObjectProperty ;
    owl:inverseOf mdhn:hasSubject ;
    rdfs:domain  mdhn:SubjectTerm;
    rdfs:range mdhn:VisualArtwork ;
    rdfs:label "has relates to"@en ;
    rdfs:comment "Associates subject to  visual artworks"@en .

 

mdhn:iiifManifest a owl:DatatypeProperty ;
    rdfs:domain mdhn:VisualArtwork ;
    rdfs:range schema:URL ;
    rdfs:label "IIIF manifest"@en ;
    rdfs:comment "Provides the URL to the IIIF manifest for the visual artwork."@en .

mdhn:iiifImage a owl:DatatypeProperty ;
    rdfs:domain mdhn:VisualArtwork ;
    rdfs:range xsd:string ;
    rdfs:label "IIIF image"@en ;
    rdfs:comment "Provides the URL to the IIIF image for the visual artwork."@en .  
